Consistency

Risc0/Gadgets/OneHot/Witness/WeakestPreFull.lean
@@ -8,131 +8,91 @@ def start_state (input: Felt) (st: State) :=
   st.WellFormed ∧
   ⟨"input"⟩ ∈ st.vars ∧
   ⟨"output"⟩ ∈ st.vars ∧
-  (st.buffers.get! ⟨"input"⟩).last! = [some input] ∧
-  (st.buffers.get! ⟨"output"⟩).last! = [none, none, none]
+  -- State.bufferWidths st { name := "input" } = some 1 ∧
+  -- st.bufferWidths[(⟨"output"⟩ : BufferVar)] = some 3 ∧
+  -- (State.buffers st (⟨"input"⟩ : BufferVar)).isSome = true ∧
+  -- (State.buffers st (⟨"input"⟩ : BufferVar)).get!.last! = [some input] ∧
+  -- List.get! (State.buffers st (⟨"input"⟩ : BufferVar)).get! st.cycle = [some input] ∧
+  (st.buffers[(⟨"output"⟩ : BufferVar)]).get!.last! = [none, none, none]
+  -- (st.buffers[(⟨"output"⟩ : BufferVar)]).get
+
+-- lemma temp (h: st.bufferWidths[({ name := "input" } : BufferVar)]! = some 1) : State.bufferWidths st { name := "input" } = some 1 := by
+--   exact h
+
+-- lemma temp2 {width : ℕ} (h: st.bufferWidths[({ name := "input" } : BufferVar)]! = some width) (hw: width > 0) : (0 <
+--     match State.bufferWidths st { name := "input" } with
+--     | some x => x
+--     | none => panicWithPosWithDecl "Init.Data.Option.BasicAux" "Option.get!" 16 14 "value is none") := by
+--   simp? [getElem!_impl_getElem, h, hw]
+--   have h1: State.bufferWidths st { name := "input"} = some width := h
+
+lemma get_from_pre (input : Felt) (st: State) (h_pre: start_state input st) :
+  0 ≤ st.cycle ∧
+    { name := "input" } ∈ st.vars ∧
+      (0 <
+          match State.bufferWidths st { name := "input" } with
+          | some x => x
+          | none =>
+            panicWithPosWithDecl "Init.Data.Option.BasicAux" "Option.get!" 16 14
+              "value is none") ∧
+        Option.isSome
+            (List.get!
+              (List.get!
+                (match State.buffers st { name := "input" } with
+                | some x => x
+                | none =>
+                  panicWithPosWithDecl "Init.Data.Option.BasicAux" "Option.get!" 16 14
+                    "value is none")
+                (Buffer.Idx.time (st.cycle - Back.toNat 0, 0)))
+              (Buffer.Idx.data (st.cycle - Back.toNat 0, 0))) =
+          true := by
+  unfold start_state at h_pre
+  simp [zero_le, ge_iff_le, forall_true_left, true_and, h_pre, Map.getElem_def, Buffer.Idx.time, Buffer.Idx.data, Back.toNat]
+  sorry
+  
+  -- MLIR_states_updates
+  -- rewrite [h_pre.right.right.right.left]
+  
 
 lemma closed_form {st: State} {input: Felt} {output₀ output₁ output₂ : Option Felt} :
   start_state input st → (
     Code.run st = [output₀, output₁, output₂] ↔ sorry
   ) := by
-  sorry
-  -- unfold start_state
-  -- intro h_pre
-  -- unfold Code.run MLIR.runProgram; simp only [Code.parts_combine]
-  -- rewrite [part₀_wp]
-  -- rewrite [part₁_updates_opaque]
-  -- rewrite [part₂_updates_opaque]
-  -- rewrite [part₃_updates_opaque]
-  -- rewrite [part₄_updates_opaque]
-  -- rewrite [part₅_updates_opaque]
-  -- rewrite [part₆_updates_opaque]
-  -- rewrite [part₇_updates_opaque]
-  -- rewrite [part₈_updates_opaque]
+  intro h_pre
+  unfold start_state at h_pre
+  rewrite [part₀_wp]
+  rewrite [part₁_updates_opaque]
+  rewrite [part₂_updates_opaque]
+  rewrite [part₃_updates_opaque]
+  rewrite [part₄_updates_opaque]
+  rewrite [part₅_updates_opaque]
+  rewrite [part₆_updates_opaque]
+  rewrite [part₇_updates_opaque]
+  rewrite [part₈_updates_opaque]
 
-  -- unfold part₀_state
-  -- simp [
-  --   h_pre, State.updateFelts, Map.get!, Option.get!, Buffer.get!,
-  --   State.set!, State.setBufferElementImpl, State.set!, Buffer.set?,
-  --   Option.isEqSome, List.set
-  -- ]
-  -- MLIR_decide_updates; simp only [Map.update_def.symm]
+  unfold part₀_state
+  MLIR_states_updates
+  simp [zero_le, ge_iff_le, forall_true_left, true_and, h_pre, Map.getElem_def, Buffer.Idx.time, Buffer.Idx.data, Back.toNat]
+  sorry
+
 
   -- unfold part₁_state
-  -- simp [
-  --   h_pre, State.updateFelts, Map.get!, Option.get!, Buffer.get!,
-  --   State.set!, State.setBufferElementImpl, State.set!, Buffer.set?,
-  --   Option.isEqSome, List.set
-  -- ]
-  -- MLIR_decide_updates; simp only [Map.update_def.symm]
+  -- MLIR_states_updates
 
   -- unfold part₂_state
-  -- simp [
-  --   h_pre, State.updateFelts, Map.get!, Option.get!, Buffer.get!,
-  --   State.set!, State.setBufferElementImpl, State.set!, Buffer.set?,
-  --   Option.isEqSome, List.set
-  -- ]
-  -- MLIR_decide_updates; simp only [Map.update_def.symm]
+  -- MLIR_states_updates
 
   -- unfold part₃_state
-  -- simp [
-  --   h_pre, State.updateFelts, Map.get!, Option.get!, Buffer.get!,
-  --   State.set!, State.setBufferElementImpl, State.set!, Buffer.set?,
-  --   Option.isEqSome, List.set
-  -- ]
-  -- MLIR_decide_updates; simp only [Map.update_def.symm]
+  -- MLIR_states_updates
 
   -- unfold part₄_state
-  -- simp [
-  --   h_pre, State.updateFelts, Map.get!, Option.get!, Buffer.get!,
-  --   State.set!, State.setBufferElementImpl, State.set!, Buffer.set?,
-  --   Option.isEqSome, List.set
-  -- ]
-  -- MLIR_decide_updates; simp only [Map.update_def.symm]
+  -- MLIR_states_updates
 
-  -- unfold part₅_state
-  -- simp [
-  --   h_pre, State.updateFelts, Map.get!, Option.get!, Buffer.get!,
-  --   State.set!, State.setBufferElementImpl, State.set!, Buffer.set?,
-  --   Option.isEqSome, List.set
-  -- ]
-  -- MLIR_decide_updates; simp only [Map.update_def.symm]
+  -- unfold part₅_state_update
+  -- MLIR_states_updates
 
-  -- unfold part₆_state
-  -- simp [
-  --   h_pre, State.updateFelts, Map.get!, Option.get!, Buffer.get!,
-  --   State.set!, State.setBufferElementImpl, State.set!, Buffer.set?,
-  --   Option.isEqSome, List.set
-  -- ]
-  -- MLIR_decide_updates; simp only [Map.update_def.symm]
-
-  -- unfold part₇_state
-  -- simp [
-  --   h_pre, State.updateFelts, Map.get!, Option.get!, Buffer.get!,
-  --   State.set!, State.setBufferElementImpl, State.set!, Buffer.set?,
-  --   Option.isEqSome, List.set
-  -- ]
-  -- MLIR_decide_updates; simp only [Map.update_def.symm]
-
-  -- unfold part₈_state
-  -- simp [
-  --   h_pre, State.updateFelts, Map.get!, Option.get!, Buffer.get!,
-  --   State.set!, State.setBufferElementImpl, State.set!, Buffer.set?,
-  --   Option.isEqSome, List.set
-  -- ]
-  -- MLIR_decide_updates; simp only [Map.update_def.symm]
-
-  -- MLIR_decide_updates; simp only [Map.update_def.symm]
-
-  -- rw [State.felts_if] <;> try rfl
-  -- simp [h_pre, State.felts]
-  -- MLIR_decide_updates; simp only [Map.update_def.symm]
-
-  -- rw [State.buffers_if] <;> try rfl
-  -- simp [h_pre, State.buffers]
-  -- MLIR_decide_updates; simp only [Map.update_def.symm]
-
-  -- rw [State.bufferWidths_if] <;> try rfl
-  -- simp [h_pre, State.bufferWidths]
-  -- MLIR_decide_updates; simp only [Map.update_def.symm]
-
-  -- rw [State.cycle_if] <;> try rfl
-  -- simp [h_pre, State.cycle]
-  -- MLIR_decide_updates; simp only [Map.update_def.symm]
-
-  -- rw [State.isFailed_if] <;> try rfl
-  -- simp [h_pre, State.isFailed]
-  -- MLIR_decide_updates; simp only [Map.update_def.symm]
-
-  -- rw [State.props_if] <;> try rfl
-  -- simp [h_pre, State.props]
-  -- MLIR_decide_updates; simp only [Map.update_def.symm]
-
-  -- rw [State.vars_if] <;> try rfl
-  -- simp [h_pre, State.vars]
-  -- MLIR_decide_updates; simp only [Map.update_def.symm]
-  
-  -- rw [State.buffers_if] <;> try rfl
-  -- simp [h_pre, State.buffers]
-  -- MLIR_decide_updates; simp only [Map.update_def.symm]
+  -- simp [State.lastOutput, Option.get!, List.getLast!, List.getLast, State.buffers]
+  -- MLIR_states_updates
+  -- simp [List.getLast]
 
 end Risc0.OneHot.Witness.WP
