Risc0.lean
@@ -3,8 +3,22 @@ import Risc0.CompoundTypes
 import Risc0.Lemmas
 import Risc0.Map
 import Risc0.Wheels
--- import Risc0.Gadgets.IsZero.Axioms
--- import Risc0.Gadgets.IsZero.Proofs
+import Risc0.Gadgets.IsZero.Constraints.Code
+import Risc0.Gadgets.IsZero.Constraints.WeakestPresPart0
+import Risc0.Gadgets.IsZero.Constraints.WeakestPresPart1
+import Risc0.Gadgets.IsZero.Constraints.WeakestPresPart2
+import Risc0.Gadgets.IsZero.Constraints.WeakestPresPart3
+import Risc0.Gadgets.IsZero.Constraints.WeakestPresPart4
+import Risc0.Gadgets.IsZero.Constraints.WeakestPreFull
+import Risc0.Gadgets.IsZero.Witness.Code
+import Risc0.Gadgets.IsZero.Witness.WeakestPresPart0
+import Risc0.Gadgets.IsZero.Witness.WeakestPresPart1
+import Risc0.Gadgets.IsZero.Witness.WeakestPresPart2
+import Risc0.Gadgets.IsZero.Witness.WeakestPresPart3
+import Risc0.Gadgets.IsZero.Witness.WeakestPresPart4
+import Risc0.Gadgets.IsZero.Witness.WeakestPresPart5
+import Risc0.Gadgets.IsZero.Witness.WeakestPreFull
+import Risc0.Gadgets.IsZero.Proofs
 import Risc0.Gadgets.OneHot.Witness.Code
 import Risc0.Gadgets.OneHot.Witness.WeakestPresPart0
 import Risc0.Gadgets.OneHot.Witness.WeakestPresPart1
