Risc0/Gadgets/IsZero/Constraints/WeakestPresPart0.lean
@@ -1,0 +1,30 @@
+import Risc0.Basic
+import Risc0.MlirTactics
+import Risc0.Gadgets.IsZero.Constraints.Code
+
+namespace Risc0.IsZero.Constraints.WP
+
+open MLIRNotation
+
+-- The state obtained by running Code.part₀ on st
+def part₀_state (st : State) : State :=
+  ((st["1"] ←ₛ some (Lit.Val 1))["0"] ←ₛ some (Lit.Val 0))["true"] ←ₛ some (Lit.Constraint True)
+
+-- Run the whole program by using part₀_state rather than Code.part₀
+def part₀_state_update (st : State) : State :=
+  Γ (part₀_state st) ⟦Code.part₁; Code.part₂; Code.part₃; Code.part₄⟧
+
+-- Prove that substituting part₀_state for Code.part₀ produces the same result
+lemma part₀_wp {st : State} :
+  Code.run st ↔
+  Code.getReturn (part₀_state_update st) := by
+  unfold Code.run MLIR.runProgram; simp only
+  rewrite [Code.parts_combine]; unfold Code.parts_combined
+  generalize eq : (Code.part₁; Code.part₂; Code.part₃; Code.part₄) = prog
+  unfold Code.part₀
+  MLIR
+  unfold part₀_state_update part₀_state
+  rewrite [←eq]
+  rfl
+
+end Risc0.IsZero.Constraints.WP
