Risc0/Gadgets/IsZero/Constraints/WeakestPresPart1.lean
@@ -1,0 +1,49 @@
+import Risc0.Basic
+import Risc0.MlirTactics
+import Risc0.Gadgets.IsZero.Constraints.Code
+import Risc0.Gadgets.IsZero.Constraints.WeakestPresPart0
+
+namespace Risc0.IsZero.Constraints.WP
+
+open MLIRNotation
+
+-- The state obtained by running Code.part₁ on st
+def part₁_state (st: State) : State := 
+  ((st["x"] ←ₛ getImpl st { name := "input" } 0 0)["out[0]"] ←ₛ
+          getImpl (st["x"] ←ₛ getImpl st { name := "input" } 0 0) { name := "output" } 0 0)["andEqz x"] ←ₛ
+        some
+          (Lit.Constraint
+            (Option.get!
+                (State.props
+                  ((st["x"] ←ₛ getImpl st { name := "input" } 0 0)["out[0]"] ←ₛ
+                    getImpl (st["x"] ←ₛ getImpl st { name := "input" } 0 0) { name := "output" } 0 0)
+                  { name := "true" }) ∧
+              Option.get!
+                  (State.felts
+                    ((st["x"] ←ₛ getImpl st { name := "input" } 0 0)["out[0]"] ←ₛ
+                      getImpl (st["x"] ←ₛ getImpl st { name := "input" } 0 0) { name := "output" } 0 0)
+                    { name := "x" }) =
+                0))
+
+-- Run the whole program by using part₁_state rather than Code.part₁
+def part₁_state_update (st: State): State :=
+  Γ (part₁_state st) ⟦Code.part₂; Code.part₃; Code.part₄⟧
+
+-- Prove that substituting part₁_state for Code.part₁ produces the same result
+lemma part₁_wp {st : State} :
+  Code.getReturn (MLIR.runProgram (Code.part₁; Code.part₂; Code.part₃; Code.part₄) st) ↔
+  Code.getReturn (part₁_state_update st) := by
+  unfold MLIR.runProgram; simp only
+  generalize eq : (Code.part₂; Code.part₃; Code.part₄) = prog
+  unfold Code.part₁
+  MLIR
+  unfold part₁_state_update part₁_state
+  rewrite [←eq]
+  rfl
+
+lemma part₁_updates_opaque {st : State} : 
+  Code.getReturn (part₀_state_update st) ↔
+  Code.getReturn (part₁_state_update (part₀_state st)) := by
+  simp [part₀_state_update, part₁_wp]
+
+end Risc0.IsZero.Constraints.WP
