Risc0/Gadgets/IsZero/Constraints/WeakestPresPart2.lean
@@ -1,0 +1,44 @@
+import Risc0.Basic
+import Risc0.MlirTactics
+import Risc0.Gadgets.IsZero.Constraints.Code
+import Risc0.Gadgets.IsZero.Constraints.WeakestPresPart1
+
+namespace Risc0.IsZero.Constraints.WP
+
+open MLIRNotation
+
+-- The state obtained by running Code.part₂ on st
+def part₂_state (st: State) : State := 
+  (State.updateFelts
+  (st["if out[0] then eqz x"] ←ₛ
+    some
+      (Lit.Constraint
+        (Option.get! (State.props st { name := "true" }) ∧
+          if Option.get! (State.felts st { name := "out[0]" }) = 0 then True
+          else Option.get! (State.props st { name := "andEqz x" }))))
+  { name := "1 - out[0]" }
+  (Option.get! (State.felts st { name := "1" }) -
+   Option.get! (State.felts st { name := "out[0]" })))["out[1]"] ←ₛ getImpl st { name := "output" } 0 1
+
+-- Run the whole program by using part₂_state rather than Code.part₂
+def part₂_state_update (st: State): State :=
+  Γ (part₂_state st) ⟦Code.part₃; Code.part₄⟧
+
+-- Prove that substituting part₂_state for Code.part₂ produces the same result
+lemma part₂_wp {st : State} :
+  Code.getReturn (MLIR.runProgram (Code.part₂; Code.part₃; Code.part₄) st) ↔
+  Code.getReturn (part₂_state_update st) := by
+  unfold MLIR.runProgram; simp only
+  generalize eq : (Code.part₃; Code.part₄) = prog
+  unfold Code.part₂
+  MLIR
+  unfold part₂_state_update part₂_state
+  rewrite [←eq]
+  rfl
+
+lemma part₂_updates_opaque {st : State} : 
+  Code.getReturn (part₁_state_update st) ↔
+  Code.getReturn (part₂_state_update (part₁_state st)) := by
+  simp [part₁_state_update, part₂_wp]
+
+end Risc0.IsZero.Constraints.WP
