Risc0/Gadgets/IsZero/Constraints/WeakestPresPart3.lean
@@ -1,0 +1,55 @@
+import Risc0.Basic
+import Risc0.MlirTactics
+import Risc0.Gadgets.IsZero.Constraints.Code
+import Risc0.Gadgets.IsZero.Constraints.WeakestPresPart2
+
+namespace Risc0.IsZero.Constraints.WP
+
+open MLIRNotation
+
+-- The state obtained by running Code.part₃ on st
+def part₃_state (st: State) : State := 
+  (State.updateFelts
+          (State.updateFelts st { name := "x * out[1]" }
+            (Option.get! (State.felts st { name := "x" }) * Option.get! (State.felts st { name := "out[1]" })))
+          { name := "x * out[1] - 1" }
+          (Option.get! (State.felts st { name := "x" }) * Option.get! (State.felts st { name := "out[1]" }) -
+            Option.get!
+              (State.felts
+                (State.updateFelts st { name := "x * out[1]" }
+                  (Option.get! (State.felts st { name := "x" }) * Option.get! (State.felts st { name := "out[1]" })))
+                { name := "1" })))["other cond"] ←ₛ
+        some
+          (Lit.Constraint
+            (Option.get! (State.props st { name := "true" }) ∧
+              Option.get! (State.felts st { name := "x" }) * Option.get! (State.felts st { name := "out[1]" }) -
+                  Option.get!
+                    (State.felts
+                      (State.updateFelts st { name := "x * out[1]" }
+                        (Option.get! (State.felts st { name := "x" }) *
+                          Option.get! (State.felts st { name := "out[1]" })))
+                      { name := "1" }) =
+                0))
+
+-- Run the whole program by using part₃_state rather than Code.part₃
+def part₃_state_update (st: State): State :=
+  Γ (part₃_state st) ⟦Code.part₄⟧
+
+-- Prove that substituting part₃_state for Code.part₃ produces the same result
+lemma part₃_wp {st : State} :
+  Code.getReturn (MLIR.runProgram (Code.part₃; Code.part₄) st) ↔
+  Code.getReturn (part₃_state_update st) := by
+  unfold MLIR.runProgram; simp only
+  generalize eq : Code.part₄ = prog
+  unfold Code.part₃
+  MLIR
+  unfold part₃_state_update part₃_state
+  rewrite [←eq]
+  rfl
+
+lemma part₃_updates_opaque {st : State} : 
+  Code.getReturn (part₂_state_update st) ↔
+  Code.getReturn (part₃_state_update (part₂_state st)) := by
+  simp [part₂_state_update, part₃_wp]
+
+end Risc0.IsZero.Constraints.WP
