Risc0/Gadgets/IsZero/Constraints/WeakestPresPart4.lean
@@ -1,0 +1,34 @@
+import Risc0.Basic
+import Risc0.MlirTactics
+import Risc0.Gadgets.IsZero.Constraints.Code
+import Risc0.Gadgets.IsZero.Constraints.WeakestPresPart3
+
+namespace Risc0.IsZero.Constraints.WP
+
+open MLIRNotation
+
+-- The state obtained by running Code.part₄ on st
+def part₄_state (st: State) : State := 
+st["if other cond"] ←ₛ
+  some
+    (Lit.Constraint
+      (Option.get! (State.props st { name := "if out[0] then eqz x" }) ∧
+        if Option.get! (State.felts st { name := "1 - out[0]" }) = 0 then True
+        else Option.get! (State.props st { name := "other cond" })))
+
+-- Prove that substituting part₄_state for Code.part₆ produces the same result
+lemma part₄_wp {st : State} :
+  Code.getReturn (MLIR.runProgram Code.part₄ st) ↔
+  Code.getReturn (part₄_state st) := by
+  unfold MLIR.runProgram; simp only
+  unfold Code.part₄
+  MLIR
+  unfold part₄_state
+  rfl
+
+lemma part₄_updates_opaque {st : State} : 
+  Code.getReturn (part₃_state_update st) ↔
+  Code.getReturn (part₄_state (part₃_state st)) := by
+  simp [part₃_state_update, part₄_wp]
+
+end Risc0.IsZero.Constraints.WP
