Risc0/Gadgets/IsZero/Proofs.lean
@@ -8,37 +8,44 @@ import Mathlib.Tactic.FieldSimp
 
 import Risc0.Basic
 import Risc0.Lemmas
-import Risc0.Gadgets.IsZero.Axioms
+import Risc0.Gadgets.IsZero.Constraints.Code
+import Risc0.Gadgets.IsZero.Constraints.WeakestPreFull
+import Risc0.Gadgets.IsZero.Witness.Code
+import Risc0.Gadgets.IsZero.Witness.WeakestPreFull
 
-namespace Risc0
+namespace Risc0.IsZero
 
 open MLIRNotation
 
-open MLIR in
-theorem is0_constraints_if_is0_witness
+theorem constraints_if_witness
   {input : Felt}
   {output : List (Option Felt)}
   (h : output.length = 2) 
   (h₁ : output.all Option.isSome) :
-  is0_witness_initial input = output → is0_constraints_initial input output := by
-  rcases output with _ | ⟨y₁, _ | ⟨y₂, ⟨_ | _⟩⟩⟩ <;> simp at *
+  -- Constraints.Code.run (Witness.Code.run (Witness.WP.start_state input)) := by
+  Witness.Code.run (Witness.WP.start_state input) = output → Constraints.Code.run (Constraints.WP.start_state input output) := by
+  rcases output with _ | ⟨y1, _ | ⟨y₂, ⟨_ | _⟩⟩⟩ <;> simp at *
   simp only [Option.isSome_iff_exists] at h₁
   rcases h₁ with ⟨⟨w₁, h₁⟩, ⟨w₂, h₂⟩⟩; subst h₁ h₂
-  rw [constraints.is0_constraints_closed_form, is0_witness_closed_form]
-  repeat split; all_goals simp [*] at *; try intros ; simp [*] at *
+  rw [Constraints.WP.closed_form, Witness.WP.closed_form]
+  repeat split; all_goals simp [*] at *; try intros; simp [*] at *
   aesop
 
-theorem is0_spec_of_constraints {x} {y₁ y₂ : Option Felt} {state : State}
-  (h : y₁.isSome) (h₁ : y₂.isSome) :
-  is0_constraints_initial x ([y₁, y₂]) → .some (.Val y₁.get!) = Op.eval {state with felts := Map.empty[⟨"x"⟩] ←ₘ x} (.Isz ⟨"x"⟩) := by
-  simp only [Option.isSome_iff_exists] at h h₁
-  rcases h with ⟨w, h⟩
-  rcases h₁ with ⟨w₁, h₁⟩
-  subst h h₁
-  rw [constraints.is0_constraints_closed_form]; aesop; aesop
-  rw [sub_eq_iff_eq_add] at h; simp [h]; aesop
-  simp [Option.get!, Map.update] at h
-  subst h
-  simp at a
+theorem spec_of_constraints {x} {y₁ y₂: Option Felt}
+  (hy₁ : y₁.isSome) (hy₂: y₂.isSome) :
+  Constraints.Code.run (Constraints.WP.start_state x ([y₁, y₂])) → (
+    x = 0 ∧ y₁ = some 1 ∨
+    x ≠ 0 ∧ y₁ = some 0 ∧ y₂ = x⁻¹
+  ) := by
+  simp only [Option.isSome_iff_exists] at hy₁
+  simp only [Option.isSome_iff_exists] at hy₂
+  rcases hy₁ with ⟨is0, hy₁_val⟩; subst y₁
+  rcases hy₂ with ⟨inv, hy₂_val⟩; subst y₂
+  rewrite [Constraints.WP.closed_form]
+  simp
+  intro hy₁ hy₂
+  simp [sub_eq_iff_eq_add, *] at *
+  aesop
+  exact Eq.symm (inv_eq_of_mul_eq_one_right hy₂)
 
-end Risc0
+end Risc0.IsZero
