Risc0/Gadgets/IsZero/Witness/WeakestPreFull.lean
@@ -1,0 +1,56 @@
+import Risc0.Gadgets.IsZero.Witness.Code
+import Risc0.Gadgets.IsZero.Witness.WeakestPresPart0
+import Risc0.Gadgets.IsZero.Witness.WeakestPresPart1
+import Risc0.Gadgets.IsZero.Witness.WeakestPresPart2
+import Risc0.Gadgets.IsZero.Witness.WeakestPresPart3
+import Risc0.Gadgets.IsZero.Witness.WeakestPresPart4
+import Risc0.Gadgets.IsZero.Witness.WeakestPresPart5
+
+namespace Risc0.IsZero.Witness.WP
+
+def start_state (input: Felt) : State :=
+  { buffers := Map.fromList [(⟨"input"⟩, [[.some input]]), (⟨"output"⟩, [[none, none]])]
+  , bufferWidths := Map.fromList [(⟨"input"⟩, 1), (⟨"output"⟩, 2)]
+  , constraints := []
+  , cycle := 0
+  , felts := Map.empty
+  , props := Map.empty
+  , vars := [⟨"input"⟩, ⟨"output"⟩]
+  , isFailed := false
+  }
+
+
+lemma closed_form {x : Felt} {y₁ y₂ : Option Felt} :
+  Code.run (start_state x) = [y₁, y₂] ↔ (.some (if x = 0 then 1 else 0)) = y₁ ∧ (if x = 0 then 0 else x⁻¹) = y₂ := by
+  rewrite [part₀_wp]
+  rewrite [part₁_updates_opaque]
+  rewrite [part₂_updates_opaque]
+  rewrite [part₃_updates_opaque]
+  rewrite [part₄_updates_opaque]
+  rewrite [part₅_updates_opaque]
+
+  unfold start_state
+
+  unfold part₀_state
+  MLIR_states_updates
+
+  unfold part₁_state
+  MLIR_states_updates
+
+  unfold part₂_state
+  MLIR_states_updates
+
+  unfold part₃_state
+  MLIR_states_updates
+
+  unfold part₄_state
+  MLIR_states_updates
+
+  unfold part₅_state
+  MLIR_states_updates
+
+  simp [State.lastOutput, Option.get!, List.getLast!, List.getLast, State.buffers]
+  MLIR_states_updates
+  simp [List.getLast]
+
+end Risc0.IsZero.Witness.WP
