Risc0/Gadgets/IsZero/Witness/WeakestPresPart1.lean
@@ -1,0 +1,40 @@
+import Risc0.Basic
+import Risc0.MlirTactics
+import Risc0.Gadgets.IsZero.Witness.Code
+import Risc0.Gadgets.IsZero.Witness.WeakestPresPart0
+
+namespace Risc0.IsZero.Witness.WP
+
+open MLIRNotation
+
+-- The state obtained by running Code.part₁ on st
+def part₁_state (st: State) : State :=
+  State.set! (State.updateFelts (State.set! (State.updateFelts st
+    { name := "isZeroBit" }
+    (if Option.get! (State.felts st { name := "x" }) = 0 then 1 else 0)) { name := "output" } 0
+    (if Option.get! (State.felts st { name := "x" }) = 0 then 1 else 0)) { name := "invVal" }
+    (if Option.get! st.felts[({ name := "x" } : FeltVar)]! = 0 then 0 else (Option.get! st.felts[({ name := "x" } : FeltVar)]!)⁻¹)) { name := "output" } 1
+    (if Option.get! st.felts[({ name := "x" } : FeltVar)]! = 0 then 0 else (Option.get! st.felts[({ name := "x" } : FeltVar)]!)⁻¹)
+
+-- Run the program from part₁ onwards by using part₁_state rather than Code.part₁
+def part₁_state_update (st: State): State :=
+  Γ (part₁_state st) ⟦Code.part₂; Code.part₃; Code.part₄; Code.part₅⟧
+
+-- Prove that substituting part₁_state for Code.part₁ produces the same result
+lemma part₁_wp {st : State} {y₁ y₂ : Option Felt} :
+  (MLIR.runProgram (Code.part₁; Code.part₂; Code.part₃; Code.part₄; Code.part₅) st).lastOutput = [y₁, y₂] ↔
+  (part₁_state_update st).lastOutput = [y₁, y₂] := by
+  unfold MLIR.runProgram; simp only
+  generalize eq : (Code.part₂; Code.part₃; Code.part₄; Code.part₅) = prog
+  unfold Code.part₁
+  MLIR
+  rewrite [←eq]
+  unfold part₁_state_update part₁_state
+  rfl
+
+lemma part₁_updates_opaque {st : State} : 
+  (part₀_state_update st).lastOutput = [y₁, y₂] ↔
+  (part₁_state_update (part₀_state st)).lastOutput = [y₁, y₂] := by
+  simp [part₀_state_update, part₁_wp]
+
+end Risc0.IsZero.Witness.WP
