Risc0/Gadgets/IsZero/Witness/WeakestPresPart2.lean
@@ -1,0 +1,35 @@
+import Risc0.Basic
+import Risc0.MlirTactics
+import Risc0.Gadgets.IsZero.Witness.Code
+import Risc0.Gadgets.IsZero.Witness.WeakestPresPart1
+
+namespace Risc0.IsZero.Witness.WP
+
+open MLIRNotation
+
+-- The state obtained by running Code.part₂ on st
+def part₂_state (st: State) : State :=
+  st["arg1[0]"] ←ₛ getImpl st { name := "output" } 0 0
+
+-- Run the program from part₂ onwards by using part₂_state rather than Code.part₂
+def part₂_state_update (st: State): State :=
+  Γ (part₂_state st) ⟦Code.part₃; Code.part₄; Code.part₅⟧
+
+-- Prove that substituting part₂_state for Code.part₂ produces the same result
+lemma part₂_wp {st : State} {y₁ y₂ : Option Felt} :
+  (MLIR.runProgram (Code.part₂; Code.part₃; Code.part₄; Code.part₅) st).lastOutput = [y₁, y₂] ↔
+  (part₂_state_update st).lastOutput = [y₁, y₂] := by
+  unfold MLIR.runProgram; simp only
+  generalize eq : (Code.part₃; Code.part₄; Code.part₅) = prog
+  unfold Code.part₂
+  MLIR
+  rewrite [←eq]
+  unfold part₂_state_update part₂_state
+  rfl
+
+lemma part₂_updates_opaque {st : State} : 
+  (part₁_state_update st).lastOutput = [y₁, y₂] ↔
+  (part₂_state_update (part₁_state st)).lastOutput = [y₁, y₂] := by
+  simp [part₁_state_update, part₂_wp]
+
+end Risc0.IsZero.Witness.WP
