Risc0/Gadgets/OneHot/Constraints/WeakestPresPart0.lean
@@ -7,32 +7,15 @@ namespace Risc0.OneHot.Constraints.WP
 open MLIRNotation
 
 -- The state obtained by running Code.part₀ on st
-def part₀_state (st: State) : State := {
-  buffers := st.buffers,
-  bufferWidths := st.bufferWidths,
-  constraints := st.constraints,
-  cycle := st.cycle,
-  felts := (State.updateFelts (State.updateFelts st { name := "1" } 1) { name := "2" } 2).felts,
-  isFailed := st.isFailed,
-  props := st.props[{ name := "true" }] ←ₘ True,
-  vars := st.vars }["input"] ←ₛ
-    if
-      0 ≤ st.cycle ∧
-      { name := "input" } ∈ st.vars ∧
-      0 < Map.get! st.bufferWidths { name := "input" } ∧
-      Option.isSome (Buffer.get! (Map.get! st.buffers { name := "input" }) (st.cycle - Back.toNat 0, 0)) =
-      true
-    then
-      some (Lit.Val (Option.get! (Buffer.get! (Map.get! st.buffers { name := "input" }) (st.cycle - Back.toNat 0, 0))))
-    else
-      none
+def part₀_state (st: State) : State :=
+  ((((st[felts][{ name := "1" }] ← 1)[felts][{ name := "2" }] ← 2)[props][{ name := "true" }] ← True)["input"] ←ₛ
+        getImpl st { name := "input" } 0 0)
 
 -- Run the whole program by using part₀_state rather than Code.part₀
 def part₀_state_update (st: State): State :=
   Γ (part₀_state st) ⟦Code.part₁; Code.part₂; Code.part₃; Code.part₄; Code.part₅; Code.part₆⟧
 
 -- Prove that substituting part₀_state for Code.part₀ produces the same result
--- ****************************** WEAKEST PRE - Part₀ ******************************
 lemma part₀_wp {st : State} :
   Code.run st ↔
   Code.getReturn (part₀_state_update st) := by
@@ -44,6 +27,5 @@ lemma part₀_wp {st : State} :
   unfold part₀_state_update part₀_state
   rewrite [←eq]
   rfl
--- ****************************** WEAKEST PRE - Part₀ ******************************
 
 end Risc0.OneHot.Constraints.WP
