Risc0/Gadgets/OneHot/Constraints/WeakestPresPart1.lean
@@ -8,149 +8,16 @@ namespace Risc0.OneHot.Constraints.WP
 open MLIRNotation
 
 -- The state obtained by running Code.part₁ on st
-def part₁_state (st: State) : State := (st["output[1]"] ←ₛ
-          if
-              0 ≤ st.cycle ∧
-                { name := "output" } ∈ st.vars ∧
-                  1 < Map.get! st.bufferWidths { name := "output" } ∧
-                    Option.isSome
-                        (Buffer.get! (Map.get! st.buffers { name := "output" }) (st.cycle - Back.toNat 0, 1)) =
-                      true then
-            some
-              (Lit.Val
-                (Option.get! (Buffer.get! (Map.get! st.buffers { name := "output" }) (st.cycle - Back.toNat 0, 1))))
-          else none)["output[2]"] ←ₛ
-        if
-            0 ≤
-                (st["output[1]"] ←ₛ
-                    if
-                        0 ≤ st.cycle ∧
-                          { name := "output" } ∈ st.vars ∧
-                            1 < Map.get! st.bufferWidths { name := "output" } ∧
-                              Option.isSome
-                                  (Buffer.get! (Map.get! st.buffers { name := "output" })
-                                    (st.cycle - Back.toNat 0, 1)) =
-                                true then
-                      some
-                        (Lit.Val
-                          (Option.get!
-                            (Buffer.get! (Map.get! st.buffers { name := "output" }) (st.cycle - Back.toNat 0, 1))))
-                    else none).cycle ∧
-              { name := "output" } ∈
-                  (st["output[1]"] ←ₛ
-                      if
-                          0 ≤ st.cycle ∧
-                            { name := "output" } ∈ st.vars ∧
-                              1 < Map.get! st.bufferWidths { name := "output" } ∧
-                                Option.isSome
-                                    (Buffer.get! (Map.get! st.buffers { name := "output" })
-                                      (st.cycle - Back.toNat 0, 1)) =
-                                  true then
-                        some
-                          (Lit.Val
-                            (Option.get!
-                              (Buffer.get! (Map.get! st.buffers { name := "output" }) (st.cycle - Back.toNat 0, 1))))
-                      else none).vars ∧
-                2 <
-                    Map.get!
-                      (st["output[1]"] ←ₛ
-                          if
-                              0 ≤ st.cycle ∧
-                                { name := "output" } ∈ st.vars ∧
-                                  1 < Map.get! st.bufferWidths { name := "output" } ∧
-                                    Option.isSome
-                                        (Buffer.get! (Map.get! st.buffers { name := "output" })
-                                          (st.cycle - Back.toNat 0, 1)) =
-                                      true then
-                            some
-                              (Lit.Val
-                                (Option.get!
-                                  (Buffer.get! (Map.get! st.buffers { name := "output" })
-                                    (st.cycle - Back.toNat 0, 1))))
-                          else none).bufferWidths
-                      { name := "output" } ∧
-                  Option.isSome
-                      (Buffer.get!
-                        (Map.get!
-                          (st["output[1]"] ←ₛ
-                              if
-                                  0 ≤ st.cycle ∧
-                                    { name := "output" } ∈ st.vars ∧
-                                      1 < Map.get! st.bufferWidths { name := "output" } ∧
-                                        Option.isSome
-                                            (Buffer.get! (Map.get! st.buffers { name := "output" })
-                                              (st.cycle - Back.toNat 0, 1)) =
-                                          true then
-                                some
-                                  (Lit.Val
-                                    (Option.get!
-                                      (Buffer.get! (Map.get! st.buffers { name := "output" })
-                                        (st.cycle - Back.toNat 0, 1))))
-                              else none).buffers
-                          { name := "output" })
-                        ((st["output[1]"] ←ₛ
-                                if
-                                    0 ≤ st.cycle ∧
-                                      { name := "output" } ∈ st.vars ∧
-                                        1 < Map.get! st.bufferWidths { name := "output" } ∧
-                                          Option.isSome
-                                              (Buffer.get! (Map.get! st.buffers { name := "output" })
-                                                (st.cycle - Back.toNat 0, 1)) =
-                                            true then
-                                  some
-                                    (Lit.Val
-                                      (Option.get!
-                                        (Buffer.get! (Map.get! st.buffers { name := "output" })
-                                          (st.cycle - Back.toNat 0, 1))))
-                                else none).cycle -
-                            Back.toNat 0,
-                          2)) =
-                    true then
-          some
-            (Lit.Val
-              (Option.get!
-                (Buffer.get!
-                  (Map.get!
-                    (st["output[1]"] ←ₛ
-                        if
-                            0 ≤ st.cycle ∧
-                              { name := "output" } ∈ st.vars ∧
-                                1 < Map.get! st.bufferWidths { name := "output" } ∧
-                                  Option.isSome
-                                      (Buffer.get! (Map.get! st.buffers { name := "output" })
-                                        (st.cycle - Back.toNat 0, 1)) =
-                                    true then
-                          some
-                            (Lit.Val
-                              (Option.get!
-                                (Buffer.get! (Map.get! st.buffers { name := "output" }) (st.cycle - Back.toNat 0, 1))))
-                        else none).buffers
-                    { name := "output" })
-                  ((st["output[1]"] ←ₛ
-                          if
-                              0 ≤ st.cycle ∧
-                                { name := "output" } ∈ st.vars ∧
-                                  1 < Map.get! st.bufferWidths { name := "output" } ∧
-                                    Option.isSome
-                                        (Buffer.get! (Map.get! st.buffers { name := "output" })
-                                          (st.cycle - Back.toNat 0, 1)) =
-                                      true then
-                            some
-                              (Lit.Val
-                                (Option.get!
-                                  (Buffer.get! (Map.get! st.buffers { name := "output" })
-                                    (st.cycle - Back.toNat 0, 1))))
-                          else none).cycle -
-                      Back.toNat 0,
-                    2))))
-        else none
+def part₁_state (st: State) : State :=
+  ((st["output[1]"] ←ₛ getImpl st { name := "output" } 0 1)["output[2]"] ←ₛ
+        getImpl (st["output[1]"] ←ₛ getImpl st { name := "output" } 0 1) { name := "output" } 0
+          2)
 
 -- Run the whole program by using part₁_state rather than Code.part₁
 def part₁_state_update (st: State): State :=
   Γ (part₁_state st) ⟦Code.part₂; Code.part₃; Code.part₄; Code.part₅; Code.part₆⟧
 
 -- Prove that substituting part₁_state for Code.part₁ produces the same result
--- ****************************** WEAKEST PRE - Part₁ ******************************
 lemma part₁_wp {st : State} :
   Code.getReturn (MLIR.runProgram (Code.part₁; Code.part₂; Code.part₃; Code.part₄; Code.part₅; Code.part₆) st) ↔
   Code.getReturn (part₁_state_update st) := by
@@ -161,7 +28,6 @@ lemma part₁_wp {st : State} :
   unfold part₁_state_update part₁_state
   rewrite [←eq]
   rfl
--- ****************************** WEAKEST PRE - Part₁ ******************************
 
 lemma part₁_updates_opaque {st : State} : 
   Code.getReturn (part₀_state_update st) ↔
