Risc0/Gadgets/OneHot/Constraints/WeakestPresPart2.lean
@@ -8,27 +8,22 @@ namespace Risc0.OneHot.Constraints.WP
 open MLIRNotation
 
 -- The state obtained by running Code.part₂ on st
-def part₂_state (st: State) : State := State.updateFelts
-        (State.updateFelts st { name := "output[2]*2" }
-          (Option.get! (State.felts st { name := "output[2]" }) * Option.get! (State.felts st { name := "2" })))
-        { name := "2*output[2]+output[1]" }
-        (Option.get!
-            (State.felts
-              (State.updateFelts st { name := "output[2]*2" }
-                (Option.get! (State.felts st { name := "output[2]" }) * Option.get! (State.felts st { name := "2" })))
+def part₂_state (st: State) : State :=
+  (st[felts][{ name := "output[2]*2" }] ←
+          Option.get! (State.felts st { name := "output[2]" }) *
+            Option.get! (State.felts st { name := "2" }))[felts][{ name := "2*output[2]+output[1]" }] ←
+        Option.get!
+            ((st.felts[{ name := "output[2]*2" }] ←ₘ
+                Option.get! (State.felts st { name := "output[2]" }) * Option.get! (State.felts st { name := "2" }))
               { name := "output[1]" }) +
-          Option.get!
-            (State.felts
-              (State.updateFelts st { name := "output[2]*2" }
-                (Option.get! (State.felts st { name := "output[2]" }) * Option.get! (State.felts st { name := "2" })))
-              { name := "output[2]*2" }))
+          Option.get! (State.felts st { name := "output[2]" }) *
+            Option.get! (State.felts st { name := "2" })
 
 -- Run the whole program by using part₂_state rather than Code.part₂
 def part₂_state_update (st: State): State :=
   Γ (part₂_state st) ⟦Code.part₃; Code.part₄; Code.part₅; Code.part₆⟧
 
 -- Prove that substituting part₂_state for Code.part₂ produces the same result
--- ****************************** WEAKEST PRE - Part₂ ******************************
 lemma part₂_wp {st : State} :
   Code.getReturn (MLIR.runProgram (Code.part₂; Code.part₃; Code.part₄; Code.part₅; Code.part₆) st) ↔
   Code.getReturn (part₂_state_update st) := by
@@ -39,7 +34,6 @@ lemma part₂_wp {st : State} :
   unfold part₂_state_update part₂_state
   rewrite [←eq]
   rfl
--- ****************************** WEAKEST PRE - Part₂ ******************************
 
 lemma part₂_updates_opaque {st : State} : 
   Code.getReturn (part₁_state_update st) ↔
