Risc0/Gadgets/OneHot/Constraints/WeakestPresPart3.lean
@@ -8,101 +8,39 @@ namespace Risc0.OneHot.Constraints.WP
 open MLIRNotation
 
 -- The state obtained by running Code.part₃ on st
-def part₃_state (st: State) : State := State.updateFelts
-        ({ buffers := st.buffers, bufferWidths := st.bufferWidths, constraints := st.constraints, cycle := st.cycle,
-            felts :=
-              (State.updateFelts st { name := "2*output[2]+output[1]-input" }
-                  (Option.get! (State.felts st { name := "2*output[2]+output[1]" }) -
-                    Option.get! (State.felts st { name := "input" }))).felts,
-            isFailed := st.isFailed,
-            props :=
-              st.props[{ name := "andEqz 2*output[2]+output[1]-input" }] ←ₘ
-                (Option.get! (State.props st { name := "true" }) ∧
-                  Option.get!
-                      (State.felts
-                        (State.updateFelts st { name := "2*output[2]+output[1]-input" }
-                          (Option.get! (State.felts st { name := "2*output[2]+output[1]" }) -
-                            Option.get! (State.felts st { name := "input" })))
-                        { name := "2*output[2]+output[1]-input" }) =
-                    0),
-            vars := st.vars }["output[0]"] ←ₛ
-          if
-              0 ≤ st.cycle ∧
-                { name := "output" } ∈ st.vars ∧
-                  0 < Map.get! st.bufferWidths { name := "output" } ∧
-                    Option.isSome
-                        (Buffer.get! (Map.get! st.buffers { name := "output" }) (st.cycle - Back.toNat 0, 0)) =
-                      true then
-            some
-              (Lit.Val
-                (Option.get! (Buffer.get! (Map.get! st.buffers { name := "output" }) (st.cycle - Back.toNat 0, 0))))
-          else none)
-        { name := "1-Output[0]" }
-        (Option.get!
+def part₃_state (st: State) : State :=
+  ((((st[felts][{ name := "2*output[2]+output[1]-input" }] ←
+              Option.get! (State.felts st { name := "2*output[2]+output[1]" }) -
+                Option.get!
+                  (State.felts st { name := "input" }))[props][{ name := "andEqz 2*output[2]+output[1]-input" }] ←
+            (Option.get! (State.props st { name := "true" }) ∧
+              Option.get! (State.felts st { name := "2*output[2]+output[1]" }) -
+                  Option.get! (State.felts st { name := "input" }) =
+                0))["output[0]"] ←ₛ
+          getImpl st { name := "output" } 0 0)[felts][{ name := "1-Output[0]" }] ←
+        Option.get!
             (State.felts
-              ({ buffers := st.buffers, bufferWidths := st.bufferWidths, constraints := st.constraints,
-                  cycle := st.cycle,
-                  felts :=
-                    (State.updateFelts st { name := "2*output[2]+output[1]-input" }
-                        (Option.get! (State.felts st { name := "2*output[2]+output[1]" }) -
-                          Option.get! (State.felts st { name := "input" }))).felts,
-                  isFailed := st.isFailed,
-                  props :=
-                    st.props[{ name := "andEqz 2*output[2]+output[1]-input" }] ←ₘ
-                      (Option.get! (State.props st { name := "true" }) ∧
-                        Option.get!
-                            (State.felts
-                              (State.updateFelts st { name := "2*output[2]+output[1]-input" }
-                                (Option.get! (State.felts st { name := "2*output[2]+output[1]" }) -
-                                  Option.get! (State.felts st { name := "input" })))
-                              { name := "2*output[2]+output[1]-input" }) =
-                          0),
-                  vars := st.vars }["output[0]"] ←ₛ
-                if
-                    0 ≤ st.cycle ∧
-                      { name := "output" } ∈ st.vars ∧
-                        0 < Map.get! st.bufferWidths { name := "output" } ∧
-                          Option.isSome
-                              (Buffer.get! (Map.get! st.buffers { name := "output" }) (st.cycle - Back.toNat 0, 0)) =
-                            true then
-                  some
-                    (Lit.Val
-                      (Option.get!
-                        (Buffer.get! (Map.get! st.buffers { name := "output" }) (st.cycle - Back.toNat 0, 0))))
-                else none)
+              (((st[felts][{ name := "2*output[2]+output[1]-input" }] ←
+                    Option.get! (State.felts st { name := "2*output[2]+output[1]" }) -
+                      Option.get!
+                        (State.felts st { name := "input" }))[props][{ name := "andEqz 2*output[2]+output[1]-input" }] ←
+                  (Option.get! (State.props st { name := "true" }) ∧
+                    Option.get! (State.felts st { name := "2*output[2]+output[1]" }) -
+                        Option.get! (State.felts st { name := "input" }) =
+                      0))["output[0]"] ←ₛ
+                getImpl st { name := "output" } 0 0)
               { name := "1" }) -
           Option.get!
             (State.felts
-              ({ buffers := st.buffers, bufferWidths := st.bufferWidths, constraints := st.constraints,
-                  cycle := st.cycle,
-                  felts :=
-                    (State.updateFelts st { name := "2*output[2]+output[1]-input" }
-                        (Option.get! (State.felts st { name := "2*output[2]+output[1]" }) -
-                          Option.get! (State.felts st { name := "input" }))).felts,
-                  isFailed := st.isFailed,
-                  props :=
-                    st.props[{ name := "andEqz 2*output[2]+output[1]-input" }] ←ₘ
-                      (Option.get! (State.props st { name := "true" }) ∧
-                        Option.get!
-                            (State.felts
-                              (State.updateFelts st { name := "2*output[2]+output[1]-input" }
-                                (Option.get! (State.felts st { name := "2*output[2]+output[1]" }) -
-                                  Option.get! (State.felts st { name := "input" })))
-                              { name := "2*output[2]+output[1]-input" }) =
-                          0),
-                  vars := st.vars }["output[0]"] ←ₛ
-                if
-                    0 ≤ st.cycle ∧
-                      { name := "output" } ∈ st.vars ∧
-                        0 < Map.get! st.bufferWidths { name := "output" } ∧
-                          Option.isSome
-                              (Buffer.get! (Map.get! st.buffers { name := "output" }) (st.cycle - Back.toNat 0, 0)) =
-                            true then
-                  some
-                    (Lit.Val
-                      (Option.get!
-                        (Buffer.get! (Map.get! st.buffers { name := "output" }) (st.cycle - Back.toNat 0, 0))))
-                else none)
+              (((st[felts][{ name := "2*output[2]+output[1]-input" }] ←
+                    Option.get! (State.felts st { name := "2*output[2]+output[1]" }) -
+                      Option.get!
+                        (State.felts st { name := "input" }))[props][{ name := "andEqz 2*output[2]+output[1]-input" }] ←
+                  (Option.get! (State.props st { name := "true" }) ∧
+                    Option.get! (State.felts st { name := "2*output[2]+output[1]" }) -
+                        Option.get! (State.felts st { name := "input" }) =
+                      0))["output[0]"] ←ₛ
+                getImpl st { name := "output" } 0 0)
               { name := "output[0]" }))
 
 -- Run the whole program by using part₃_state rather than Code.part₃
@@ -110,7 +48,6 @@ def part₃_state_update (st: State): State :=
   Γ (part₃_state st) ⟦Code.part₄; Code.part₅; Code.part₆⟧
 
 -- Prove that substituting part₃_state for Code.part₃ produces the same result
--- ****************************** WEAKEST PRE - Part₃ ******************************
 lemma part₃_wp {st : State} :
   Code.getReturn (MLIR.runProgram (Code.part₃; Code.part₄; Code.part₅; Code.part₆) st) ↔
   Code.getReturn (part₃_state_update st) := by
@@ -121,7 +58,6 @@ lemma part₃_wp {st : State} :
   unfold part₃_state_update part₃_state
   rewrite [←eq]
   rfl
--- ****************************** WEAKEST PRE - Part₃ ******************************
 
 lemma part₃_updates_opaque {st : State} : 
   Code.getReturn (part₂_state_update st) ↔
