Risc0/Gadgets/OneHot/Constraints/WeakestPresPart4.lean
@@ -8,116 +8,54 @@ namespace Risc0.OneHot.Constraints.WP
 open MLIRNotation
 
 -- The state obtained by running Code.part₄ on st
-def part₄_state (st: State) : State := State.updateFelts
-        (State.updateFelts
-          { buffers := st.buffers, bufferWidths := st.bufferWidths, constraints := st.constraints, cycle := st.cycle,
-            felts :=
-              (State.updateFelts st { name := "output[0]<=1" }
-                  (Option.get! (State.felts st { name := "output[0]" }) *
-                    Option.get! (State.felts st { name := "1-Output[0]" }))).felts,
-            isFailed := st.isFailed,
-            props :=
-              st.props[{ name := "andEqz output[0]<=1" }] ←ₘ
-                (Option.get! (State.props st { name := "andEqz 2*output[2]+output[1]-input" }) ∧
-                  Option.get!
-                      (State.felts
-                        (State.updateFelts st { name := "output[0]<=1" }
-                          (Option.get! (State.felts st { name := "output[0]" }) *
-                            Option.get! (State.felts st { name := "1-Output[0]" })))
-                        { name := "output[0]<=1" }) =
-                    0),
-            vars := st.vars }
-          { name := "1-Output[1]" }
-          (Option.get!
-              (State.felts
-                (State.updateFelts st { name := "output[0]<=1" }
-                  (Option.get! (State.felts st { name := "output[0]" }) *
-                    Option.get! (State.felts st { name := "1-Output[0]" })))
+def part₄_state (st: State) : State :=
+  ((((st[felts][{ name := "output[0]<=1" }] ←
+              Option.get! (State.felts st { name := "output[0]" }) *
+                Option.get! (State.felts st { name := "1-Output[0]" }))[props][{ name := "andEqz output[0]<=1" }] ←
+            (Option.get! (State.props st { name := "andEqz 2*output[2]+output[1]-input" }) ∧
+              (Option.get! (State.felts st { name := "output[0]" }) = 0 ∨
+                Option.get! (State.felts st { name := "1-Output[0]" }) = 0)))[felts][{ name := "1-Output[1]" }] ←
+          Option.get!
+              ((st.felts[{ name := "output[0]<=1" }] ←ₘ
+                  Option.get! (State.felts st { name := "output[0]" }) *
+                    Option.get! (State.felts st { name := "1-Output[0]" }))
                 { name := "1" }) -
             Option.get!
-              (State.felts
-                (State.updateFelts st { name := "output[0]<=1" }
-                  (Option.get! (State.felts st { name := "output[0]" }) *
-                    Option.get! (State.felts st { name := "1-Output[0]" })))
-                { name := "output[1]" })))
-        { name := "output[1]<=1" }
-        (Option.get!
-            (State.felts
-              (State.updateFelts
-                { buffers := st.buffers, bufferWidths := st.bufferWidths, constraints := st.constraints,
-                  cycle := st.cycle,
-                  felts :=
-                    (State.updateFelts st { name := "output[0]<=1" }
-                        (Option.get! (State.felts st { name := "output[0]" }) *
-                          Option.get! (State.felts st { name := "1-Output[0]" }))).felts,
-                  isFailed := st.isFailed,
-                  props :=
-                    st.props[{ name := "andEqz output[0]<=1" }] ←ₘ
-                      (Option.get! (State.props st { name := "andEqz 2*output[2]+output[1]-input" }) ∧
-                        Option.get!
-                            (State.felts
-                              (State.updateFelts st { name := "output[0]<=1" }
-                                (Option.get! (State.felts st { name := "output[0]" }) *
-                                  Option.get! (State.felts st { name := "1-Output[0]" })))
-                              { name := "output[0]<=1" }) =
-                          0),
-                  vars := st.vars }
-                { name := "1-Output[1]" }
-                (Option.get!
-                    (State.felts
-                      (State.updateFelts st { name := "output[0]<=1" }
-                        (Option.get! (State.felts st { name := "output[0]" }) *
-                          Option.get! (State.felts st { name := "1-Output[0]" })))
+              ((st.felts[{ name := "output[0]<=1" }] ←ₘ
+                  Option.get! (State.felts st { name := "output[0]" }) *
+                    Option.get! (State.felts st { name := "1-Output[0]" }))
+                { name := "output[1]" }))[felts][{ name := "output[1]<=1" }] ←
+        Option.get!
+            (((st.felts[{ name := "output[0]<=1" }] ←ₘ
+                  Option.get! (State.felts st { name := "output[0]" }) *
+                    Option.get! (State.felts st { name := "1-Output[0]" }))[{ name := "1-Output[1]" }] ←ₘ
+                Option.get!
+                    ((st.felts[{ name := "output[0]<=1" }] ←ₘ
+                        Option.get! (State.felts st { name := "output[0]" }) *
+                          Option.get! (State.felts st { name := "1-Output[0]" }))
                       { name := "1" }) -
                   Option.get!
-                    (State.felts
-                      (State.updateFelts st { name := "output[0]<=1" }
-                        (Option.get! (State.felts st { name := "output[0]" }) *
-                          Option.get! (State.felts st { name := "1-Output[0]" })))
-                      { name := "output[1]" })))
+                    ((st.felts[{ name := "output[0]<=1" }] ←ₘ
+                        Option.get! (State.felts st { name := "output[0]" }) *
+                          Option.get! (State.felts st { name := "1-Output[0]" }))
+                      { name := "output[1]" }))
               { name := "output[1]" }) *
-          Option.get!
-            (State.felts
-              (State.updateFelts
-                { buffers := st.buffers, bufferWidths := st.bufferWidths, constraints := st.constraints,
-                  cycle := st.cycle,
-                  felts :=
-                    (State.updateFelts st { name := "output[0]<=1" }
-                        (Option.get! (State.felts st { name := "output[0]" }) *
-                          Option.get! (State.felts st { name := "1-Output[0]" }))).felts,
-                  isFailed := st.isFailed,
-                  props :=
-                    st.props[{ name := "andEqz output[0]<=1" }] ←ₘ
-                      (Option.get! (State.props st { name := "andEqz 2*output[2]+output[1]-input" }) ∧
-                        Option.get!
-                            (State.felts
-                              (State.updateFelts st { name := "output[0]<=1" }
-                                (Option.get! (State.felts st { name := "output[0]" }) *
-                                  Option.get! (State.felts st { name := "1-Output[0]" })))
-                              { name := "output[0]<=1" }) =
-                          0),
-                  vars := st.vars }
-                { name := "1-Output[1]" }
-                (Option.get!
-                    (State.felts
-                      (State.updateFelts st { name := "output[0]<=1" }
-                        (Option.get! (State.felts st { name := "output[0]" }) *
-                          Option.get! (State.felts st { name := "1-Output[0]" })))
-                      { name := "1" }) -
-                  Option.get!
-                    (State.felts
-                      (State.updateFelts st { name := "output[0]<=1" }
-                        (Option.get! (State.felts st { name := "output[0]" }) *
-                          Option.get! (State.felts st { name := "1-Output[0]" })))
-                      { name := "output[1]" })))
-              { name := "1-Output[1]" }))
+          (Option.get!
+              ((st.felts[{ name := "output[0]<=1" }] ←ₘ
+                  Option.get! (State.felts st { name := "output[0]" }) *
+                    Option.get! (State.felts st { name := "1-Output[0]" }))
+                { name := "1" }) -
+            Option.get!
+              ((st.felts[{ name := "output[0]<=1" }] ←ₘ
+                  Option.get! (State.felts st { name := "output[0]" }) *
+                    Option.get! (State.felts st { name := "1-Output[0]" }))
+                { name := "output[1]" })))
 
 -- Run the whole program by using part₄_state rather than Code.part₄
 def part₄_state_update (st: State): State :=
   Γ (part₄_state st) ⟦Code.part₅; Code.part₆⟧
 
 -- Prove that substituting part₄_state for Code.part₄ produces the same result
--- ****************************** WEAKEST PRE - Part₄ ******************************
 lemma part₄_wp {st : State} :
   Code.getReturn (MLIR.runProgram (Code.part₄; Code.part₅; Code.part₆) st) ↔
   Code.getReturn (part₄_state_update st) := by
@@ -128,7 +66,6 @@ lemma part₄_wp {st : State} :
   unfold part₄_state_update part₄_state
   rewrite [←eq]
   rfl
--- ****************************** WEAKEST PRE - Part₄ ******************************
 
 lemma part₄_updates_opaque {st : State} : 
   Code.getReturn (part₃_state_update st) ↔
