Risc0/Gadgets/OneHot/Witness/WeakestPresPart0.lean
@@ -7,16 +7,16 @@ namespace Risc0.OneHot.Witness.WP
 open MLIRNotation
 
 -- The state obtained by running Code.part₀ on st
-def part₀_state (st: State) : State := (((st[felts][{ name := "2" }] ← 2)[felts][{ name := "1" }] ← 1)[felts][{ name := "0" }] ← 0)["input"] ←ₛ
+def part₀_state (st: State) : State :=
+  ((((st[felts][{ name := "2" }] ← 2)[felts][{ name := "1" }] ← 1)[felts][{ name := "0" }] ← 0)["input"] ←ₛ
           getImpl st { name := "input" } 0
-            0
+            0)
 
 -- Run the whole program by using part₀_state rather than Code.part₀
 def part₀_state_update (st: State): State :=
   Γ (part₀_state st) ⟦Code.part₁; Code.part₂; Code.part₃; Code.part₄; Code.part₅; Code.part₆; Code.part₇; Code.part₈⟧
 
 -- Prove that substituting part₀_state for Code.part₀ produces the same result
--- ****************************** WEAKEST PRE - Part₀ ******************************
 lemma part₀_wp {st : State} {y₁ y₂ y₃ : Option Felt} :
   Code.run st = [y₁, y₂, y₃] ↔
   (part₀_state_update st).lastOutput = [y₁, y₂, y₃] := by
@@ -28,6 +28,5 @@ lemma part₀_wp {st : State} {y₁ y₂ y₃ : Option Felt} :
   unfold part₀_state_update part₀_state
   rewrite [←eq]
   rfl
--- ****************************** WEAKEST PRE - Part₀ ******************************
 
 end Risc0.OneHot.Witness.WP
