Risc0/Gadgets/OneHot/Witness/WeakestPresPart1.lean
@@ -9,7 +9,7 @@ open MLIRNotation
 
 -- The state obtained by running Code.part₁ on st
 def part₁_state (st: State) : State :=
-  (State.set!
+  ((State.set!
               (st[felts][{ name := "input == 0" }] ←
                 if Option.get! (State.felts st { name := "input" }) = 0 then 1 else 0)
               { name := "output" } 0
@@ -33,14 +33,13 @@ def part₁_state (st: State) : State :=
                       { name := "1" }) =
                 0 then
             1
-          else 0
+          else 0)
 
 -- Run the program from part₁ onwards by using part₁_state rather than Code.part₁
 def part₁_state_update (st: State): State :=
   Γ (part₁_state st) ⟦Code.part₂; Code.part₃; Code.part₄; Code.part₅; Code.part₆; Code.part₇; Code.part₈⟧
 
 -- Prove that substituting part₁_state for Code.part₁ produces the same result
--- ****************************** WEAKEST PRE - Part₁ ******************************
 lemma part₁_wp {st : State} {y₁ y₂ y₃ : Option Felt} :
   (MLIR.runProgram (Code.part₁; Code.part₂; Code.part₃; Code.part₄; Code.part₅; Code.part₆; Code.part₇; Code.part₈) st).lastOutput = [y₁, y₂, y₃] ↔
   (part₁_state_update st).lastOutput = [y₁, y₂, y₃] := by
@@ -51,7 +50,6 @@ lemma part₁_wp {st : State} {y₁ y₂ y₃ : Option Felt} :
   rewrite [←eq]
   unfold part₁_state_update part₁_state
   rfl
--- ****************************** WEAKEST PRE - Part₁ ******************************
 
 lemma part₁_updates_opaque {st : State} : 
   (part₀_state_update st).lastOutput = [y₁, y₂, y₃] ↔
