Risc0/Gadgets/OneHot/Witness/WeakestPresPart3.lean
@@ -9,16 +9,15 @@ open MLIRNotation
 
 -- The state obtained by running Code.part₃ on st
 def part₃_state (st: State) : State :=
-  (st["output[1]"] ←ₛ getImpl st { name := "output" } 0 1)["output[2]"] ←ₛ
+  ((st["output[1]"] ←ₛ getImpl st { name := "output" } 0 1)["output[2]"] ←ₛ
           getImpl (st["output[1]"] ←ₛ getImpl st { name := "output" } 0 1) { name := "output" } 0
-            2
+            2)
 
 -- Run the program from part₃ onwards by using part₃_state rather than Code.part₃
 def part₃_state_update (st: State): State :=
   Γ (part₃_state st) ⟦Code.part₄; Code.part₅; Code.part₆; Code.part₇; Code.part₈⟧
 
 -- Prove that substituting part₃_state for Code.part₃ produces the same result
--- ****************************** WEAKEST PRE - Part₃ ******************************
 lemma part₃_wp {st : State} {y₁ y₂ y₃ : Option Felt} :
   (MLIR.runProgram (Code.part₃; Code.part₄; Code.part₅; Code.part₆; Code.part₇; Code.part₈) st).lastOutput = [y₁, y₂, y₃] ↔
   (part₃_state_update st).lastOutput = [y₁, y₂, y₃] := by
@@ -29,7 +28,6 @@ lemma part₃_wp {st : State} {y₁ y₂ y₃ : Option Felt} :
   rewrite [←eq]
   unfold part₃_state_update part₃_state
   rfl
--- ****************************** WEAKEST PRE - Part₃ ******************************
 
 lemma part₃_updates_opaque {st : State} : 
   (part₂_state_update st).lastOutput = [y₁, y₂, y₃] ↔
