Risc0/Gadgets/OneHot/Witness/WeakestPresPart5.lean
@@ -8,8 +8,8 @@ namespace Risc0.OneHot.Witness.WP
 open MLIRNotation
 
 -- The state obtained by running Code.part₅ on st
-def part₅_state (st: State) : State := {
-  buffers := (st["output[0]"] ←ₛ getImpl st { name := "output" } 0 0).buffers,
+def part₅_state (st: State) : State :=
+  { buffers := (st["output[0]"] ←ₛ getImpl st { name := "output" } 0 0).buffers,
           bufferWidths := (st["output[0]"] ←ₛ getImpl st { name := "output" } 0 0).bufferWidths,
           constraints :=
             (Option.get!
@@ -54,7 +54,6 @@ def part₅_state_update (st: State): State :=
   Γ (part₅_state st) ⟦Code.part₆; Code.part₇; Code.part₈⟧
 
 -- Prove that substituting part₅_state for Code.part₅ produces the same result
--- ****************************** WEAKEST PRE - Part₅ ******************************
 lemma part₅_wp {st : State} {y₁ y₂ y₃ : Option Felt} :
   (MLIR.runProgram (Code.part₅; Code.part₆; Code.part₇; Code.part₈) st).lastOutput = [y₁, y₂, y₃] ↔
   (part₅_state_update st).lastOutput = [y₁, y₂, y₃] := by
@@ -65,7 +64,6 @@ lemma part₅_wp {st : State} {y₁ y₂ y₃ : Option Felt} :
   rewrite [←eq]
   unfold part₅_state_update part₅_state
   rfl
--- ****************************** WEAKEST PRE - Part₅ ******************************
 
 lemma part₅_updates_opaque {st : State} : 
   (part₄_state_update st).lastOutput = [y₁, y₂, y₃] ↔
